feat: elaboration overview (#41)

Manual/Elaboration.lean
@@ -6,27 +6,432 @@ open Verso.Genre Manual
 
 set_option pp.rawOnError true
 
-#doc (Manual) "Elaboration, Evaluation, and Compilation" =>
-
-:::planned
+open Lean (Syntax SourceInfo)
 
 
- * Describe the roles of the {deftech}_kernel_, the interpreter, the compiler, the {deftech}[elaborator], and how they interact
- * Sketch the pipeline (parser -> command elaborator (with macro expansion) -> term elaborator (with macro expansion) -> ...
- * Cost model for programs - what data is present at which stage?
+def pratt73 : InProceedings where
+  title := .concat (inlines!"Top down operator precedence")
+  authors := #[.concat (inlines!"Vaughan Pratt")]
+  year := 1973
+  booktitle := .concat (inlines!"Proceedings of the 1st Annual ACM SIGACT-SIGPLAN Symposium on Principles of Programming Languages")
+
+def carneiro19 : Thesis where
+  title := .concat (inlines!"The Type Theory of Lean")
+  author := .concat (inlines!"Mario Carneiro")
+  year := 2019
+  university := .concat (inlines!"Carnegie Mellon University")
+  url := some "https://github.com/digama0/lean-type-theory/releases/download/v1.0/main.pdf"
+  degree := .concat (inlines!"Masters thesis")
+
+def ullrich23 : Thesis where
+  title := .concat (inlines!"An Extensible Theorem Proving Frontend")
+  author := .concat (inlines!"Sebastian Ullrich")
+  year := 2023
+  university := .concat (inlines!"Karlsruhe Institute of Technology")
+  url := some "https://www.lean-lang.org/papers/thesis-sebastian.pdf"
+  degree := .concat (inlines!"Dr. Ing. dissertation")
+
+#doc (Manual) "Elaboration and Compilation" =>
+%%%
+htmlSplit := .never
+%%%
+
+Roughly speaking, Lean's processing of a source file can be divided into the following stages:
+
+: Parsing
+
+  The parser transforms sequences of characters into syntax trees of type {lean}`Syntax`.
+  Lean's parser is extensible, so the {lean}`Syntax` datatype is very general.
+
+: Macro Expansion
+
+  Macros are transformations that replace syntactic sugar with more basic syntax.
+  Both the input and output of macro expansion have type {lean}`Syntax`.
+
+: Elaboration
+
+  {deftech key:="elaborator"}[Elaboration] is the process of transforming Lean's user-facing syntax into its core type theory.
+  This core theory is much simpler, enabling the trusted kernel to be very small.
+  Elaboration additionally produces metadata, such as proof states or the types of expressions, used for Lean's interactive features, storing them in a side table.
+
+: Kernel Checking
+
+  Lean's trusted kernel checks the output of the elaborator to ensure that it follows the rules of the type theory.
+
+: Compilation
+
+  The compiler transforms elaborated Lean code into executables that can be run.
+
+
+:::figure "The Lean Pipeline" (name := "pipeline-overview")
+![The Lean Pipeline](/static/figures/pipeline-overview.svg)
 :::
+
+
+In reality, the stages described above do not strictly occur one after the other.
+Lean parses a single {tech}[command] (top-level declaration), elaborates it, and performs any necessary kernel checks.
+Macro expansion is part of elaboration; before translating a piece of syntax, the elaborator first expands any macros present at the outermost layer.
+Macro syntax may remain at deeper layers, but it will be expanded when the elaborator reaches those layers.
+There are multiple kinds of elaboration: command elaboration implements the effects of each top-level command (e.g. declaring datatypes, saving definitions, evaluating expressions), while term elaboration is responsible for constructing the terms that occur in many commands (e.g. types in signatures, the right-hand sides of definitions, or expressions to be evaluated).
+Tactic execution is a specialization of term elaboration.
+
+When a command is elaborated, the state of Lean changes.
+New definitions or types may have been saved for future use, the syntax may be extended, or the set of names that can be referred to without explicit qualification may have changed.
+The next command is parsed and elaborated in this updated state, and itself updates the state for subsequent commands.
+
+# Parsing
+
+Lean's parser is a recursive-descent parser that uses dynamic tables based on Pratt parsing{citep pratt73}[] to resolve operator precedence and associativity.
+When grammars are unambiguous, the parser does not need to backtrack; in the case of ambiguous grammars, a memoization table similar to that used in Packrat parsing avoids exponential blowup.
+Parsers are highly extensible: users may define new syntax in any command, and that syntax becomes available in the next command.
+The open namespaces in the current {tech}[scope] also influences which parsing rules are used, because parser extensions may be set to be active only when a given namespace is open.
+
+When ambiguity is encountered, the longest matching parse is selected.
+If there is no unique longest match, then both matching parses are saved in the syntax tree in a {deftech}[choice node] to be resolved later by the elaborator.
+When the parser fails, it returns a {lean}`Syntax.missing` node, allowing for error recovery.
+
+When successful, the parser saves sufficient information to reconstruct the original source file.
+Unsuccessful parses may miss some information for the regions of the file that cannot be parsed.
+The {lean}`SourceInfo` record type records information about the origin of a piece of syntax, including its source location and the surrounding whitespace.
+Based on the {lean}`SourceInfo` field, there are three relationships that {lean}`Syntax` can have to a source file:
+ * {lean}`SourceInfo.original` indicates that the syntax value was produced directly by the parser.
+ * {lean}`SourceInfo.synthetic` indicates that the syntax value was produced programmatically, e.g. by the macro expander. Synthetic syntax may nonetheless be marked _canonical_, in which case the Lean user interface treats it as if the user had written it. Synthetic syntax is annotated with positions in the original file, but does not include leading or trailing whitespace.
+ * {lean}`SourceInfo.none` indicates no relationship to a file.
+
+The parser maintains a token table that tracks the reserved words that are currently part of the language.
+Defining new syntax or opening namespaces can cause a formerly-valid identifier to become a keyword.
+
+Each production in Lean's grammar is named.
+The name of a production is called its {deftech}_kind_.
+These syntax kinds are important, because they are the key used to look up the interpretation of the syntax in the elaborator's tables.
+
+Syntax extensions are described in more detail in {ref "language-extension"}[a dedicated chapter].
+
+# Macro Expansion and Elaboration
+
+Having parsed a command, the next step is to elaborate it.
+The precise meaning of _elaboration_ depends on what is being elaborated: elaborating a command effects a change in the state of Lean, while elaborating a term results in a term in Lean's core type theory.
+Elaboration of both commands and terms may be recursive, both because of command combinators such as {keywordOf Lean.Parser.Command.in}`in` and because terms may contain other terms.
+
+Command and term elaboration have different capabilities.
+Command elaboration may have side effects on an environment, and it has access to run arbitrary computations in {lean}`IO`.
+Lean environments contain the usual mapping from names to definitions along with additional data defined in {deftech}[environment extensions], which are additional tables associated with an environment; environment extensions are used to track most other information about Lean code, including {tactic}`simp` lemmas, custom pretty printers, and internals such as the compiler's intermediate representations.
+Command elaboration also maintains a message log with the contents of the compiler's informational output, warnings, and errors, a set of {tech}[info trees] that associate metadata with the original syntax (used for interactive features such as displaying proof states, identifier completion, and showing documentation), accumulated debugging traces, the open {tech}[scopes], and some internal state related to macro expansion.
+Term elaboration may modify all of these fields except the open scopes.
+Additionally, it has access to all the machinery needed to create fully-explicit terms in the core language from Lean's terse, friendly syntax, including unification, type class instance synthesis, and type checking.
+
+The first step in both term and command elaboration is macro expansion.
+There is a table that maps syntax kinds to macro implementations; macro implementations are monadic functions that transform the macro syntax into new syntax.
+Macros are saved in the same table and execute in the same monad for terms, commands, tactics, and any other macro-extensible part of Lean.
+If the syntax returned by the macro is itself a macro, then that syntax is again expanded—this process is repeated until either a syntax whose kind is not a macro is produced, or until a maximum number of iterations is reached, at which point Lean produces an error.
+Typical macros process some outer layer of their syntax, leaving some subterms untouched.
+This means that even when macro expansion has been completed, there still may be macro invocations remaining in the syntax below the top level.
+New macros may be added to the macro table.
+Defining new macros is described in detail in {ref "macros"}[the section on macros].
+
+After macro expansion, both the term and command elaborators consult tables that map syntax kinds to elaboration procedures.
+Term elaborators map syntax and an optional expected type to a core language expression using the very featureful monad mentioned above.
+Command elaborators accept syntax and return no value, but may have monadic side effects on the global command state.
+While both term and command elaborators have access to {lean}`IO`, it's unusual that they perform side effects; exceptions include interactions with external tools or solvers.
+
+The elaborator tables may be extended to enable the use of new syntax for both terms and commands by extending the tables.
+See {ref "elaborators"}[the section on elaborators] for a description of how to add additional elaborators to Lean.
+When commands or terms contain further commands or terms, they recursively invoke the appropriate elaborator on the nested syntax.
+This elaborator will then expand macros before invoking elaborators from the table.
+While macro expansion occurs prior to elaboration for a given “layer” of the syntax, macro expansion and elaboration are interleaved in general.
+
+## Info Trees
+
+When interacting with Lean code, much more information is needed than when simply importing it as a dependency.
+For example, Lean's interactive environment can be used to view the types of selected expressions, to step through all the intermediate states of a proof, to view documentation, and highlight all occurrences of a bound variable.
+The information necessary to use Lean interactively is stored in a side table called the  {deftech}_info trees_ during elaboration.
+
+````lean (show := false)
+open Lean.Elab (Info)
+deriving instance TypeName for Unit
+````
+
+
+Info trees relate metadata to the user's original syntax.
+Their tree structure corresponds closely to the tree structure of the syntax, although a given node in the syntax tree may have many corresponding info tree nodes that document different aspects of it.
+This metadata includes the elaborator's output in Lean's core language, the proof state active at a given point, suggestions for interactive identifier completion, and much more.
+The metadata can also be arbitrarily extended; the constructor {lean}`Info.ofCustomInfo` accepts a {lean}`Dynamic` type.
+This can be used to add information to be used by custom code actions or other user interface extensions.
+
+# The Kernel
+
+Lean's trusted {deftech}_kernel_ is a small, robust implementation of a type checker for the core type theory.
+It does not include a syntactic termination checker, nor does it perform unification; termination is guaranteed by elaborating all recursive functions into uses of primitive {tech}[recursors], and unification is expected to have already been carried out by the elaborator.
+Before new inductive types or definitions are added to the environment by the command or term elaborators, they must be checked by the kernel to guard against potential bugs in elaboration.
+
+Lean's kernel is written in C++.
+There is an independent re-implementation in Rust, and the Lean project is interested in having as many implementations as possible so that they can be cross-checked against each other.
+
+The language implemented by the kernel is a version of the Calculus of Constructions, a dependent type theory with the following features:
+ * Full dependent types
+ * Inductively-defined datatypes that may be mutually inductive or include recursion nested under other inductive types
+ * An {tech}[impredicative], definitionally proof-irrelevant, extensional {tech}[universe] of {tech}[propositions]
+ * A {tech}[predicative], non-cumulative hierarchy of universes of data
+ * {ref "quotients"}[Quotient types] with a definitional computation rule
+ * Propositional function extensionality{margin}[Function extensionality is a theorem that can be proved using quotient types, but it is such an important consequence that it's worth listing separately.]
+ * Definitional η-equality for functions and products
+ * Universe-polymorphic definitions
+ * Consistency: there is no axiom-free closed term of type {lean}`False`
+
+```lean (show := false) (keep := false)
+-- Test definitional eta for structures
+structure A where
+  x : Nat
+  y : Int
+example (a : A) : ⟨a.x, a.y⟩ = a := rfl
+inductive B where
+  | mk (x : Nat) (y : Int) : B
+example (b : B) : ⟨b.1, b.2⟩ = b := rfl
+/--
+error: type mismatch
+  rfl
+has type
+  e1 = e1 : Prop
+but is expected to have type
+  e1 = e2 : Prop
+-/
+#guard_msgs in
+example (e1 e2 : Empty) : e1 = e2 := rfl
+```
+
+This theory is rich enough to express leading-edge research mathematics, and yet simple enough to admit a small, efficient implementation.
+The presence of explicit proof terms makes it feasible to implement independent proof checkers, increasing our confidence.
+It is described in detail by {citet carneiro19}[] and {citet ullrich23}[].
+
+Lean's type theory does not feature subject reduction, the definitional equality is not necessarily transitive, and it is possible to make the type checker fail to terminate.
+None of these metatheoretic properties cause problems in practice—failures of transitivity are exceedingly rare, and as far as we know, nontermination has not occurred except when crafting code specifically to exercise it.
+Most importantly, logical soundness is not affected.
+In practice, apparent nontermination is indistinguishable from sufficiently slow programs; the latter are the causes observed in the wild.
+These metatheoretic properties are a result of having impredicativity, quotient types that compute, definitional proof irrelevance, and propositional extensionality; these features are immensely valuable both to support ordinary mathematical practice and to enable automation.
+
+# Elaboration Results
+
+Lean's core type theory does not include pattern matching or recursive definitions.
+Instead, it provides low-level {tech}[recursors] that can be used to implement both case distinction and primitive recursion.
+Thus, the elaborator must translate definitions that use pattern matching and recursion into definitions that use recursors.
+This translation is additionally a proof that the function terminates for all potential arguments, because all functions that can be translated to recursors also terminate.
+
+The translation to recursors happens in two phases: during term elaboration, uses of pattern matching are replaced by appeals to auxiliary functions that implement the particular case distinction that occurs in the code.
+These auxiliary functions are themselves defined using recursors, though they do not make use of the recursors' ability to actually implement recursive behavior.{margin}[They use the `casesOn` construction that is described in the {ref "recursor-elaboration-helpers"}[section on recursors and elaboration].]
+The term elaborator thus returns core-language terms in which pattern matching has been replaced with the use of special functions that implement case distinction, but these terms may still contain recursive occurrences of the function being defined.
+To see auxiliary pattern matching functions in Lean's output, set the option {option}`pp.match` to {lean}`false`.
+
+{optionDocs pp.match}
+
+
+```lean (show := false) (keep := false)
+def third_of_five : List α → Option α
+  | [_, _, x, _, _] => some x
+  | _ => none
+set_option pp.match false
+/--
+info: third_of_five.eq_def.{u_1} {α : Type u_1} :
+  ∀ (x : List α),
+    third_of_five x = third_of_five.match_1 (fun x => Option α) x (fun head head x head head => some x) fun x => none
+-/
+#guard_msgs in
+#check third_of_five.eq_def
+/--
+info: def third_of_five.match_1.{u_1, u_2} : {α : Type u_1} →
+  (motive : List α → Sort u_2) →
+    (x : List α) →
+      ((head head_1 x head_2 head_3 : α) → motive [head, head_1, x, head_2, head_3]) →
+        ((x : List α) → motive x) → motive x :=
+fun {α} motive x h_1 h_2 =>
+  List.casesOn x (h_2 []) fun head tail =>
+    List.casesOn tail (h_2 [head]) fun head_1 tail =>
+      List.casesOn tail (h_2 [head, head_1]) fun head_2 tail =>
+        List.casesOn tail (h_2 [head, head_1, head_2]) fun head_3 tail =>
+          List.casesOn tail (h_2 [head, head_1, head_2, head_3]) fun head_4 tail =>
+            List.casesOn tail (h_1 head head_1 head_2 head_3 head_4) fun head_5 tail =>
+              h_2 (head :: head_1 :: head_2 :: head_3 :: head_4 :: head_5 :: tail)
+-/
+#guard_msgs in
+#print third_of_five.match_1
+```
+
+The elaborated definition is then sent to the compiler and to the kernel.
+The compiler receives the version in which recursion is still present, while the version sent to the kernel undergoes a second transformation that replaces explicit recursion with uses of recursors.
+This split is for three reasons:
+ * The compiler can compile {ref "partial-unsafe"}[`partial` functions] that the kernel treats as opaque constants for the purposes of reasoning.
+ * The compiler can also compile {ref "partial-unsafe"}[`unsafe` functions] that bypass the kernel entirely.
+ * Translation to recursors does not necessarily preserve the cost model expected by programmers, in particular laziness vs strictness, but compiled code must have predictable performance.
+The compiler stores an intermediate representation in an environment extension.
+
+For straightforwardly structurally recursive functions, the translation will use the datatype's recursor.
+These functions tend to be relatively efficient when run in the kernel, their defining equations hold definitionally, and they are easy to understand.
+Functions that use other patterns of recursion that cannot be captured by the datatype's recursor are translated using {deftech}[well-founded recursion], which is structural recursion on a proof that some measure decreases at each recursive call.
+Lean can automatically derive many of these cases, but some require manual proofs.
+Well-founded recursion is more flexible, but the resulting functions are often slower to execute in the kernel due to the proof terms that show that a measure decreases, and their defining equations may hold only propositionally.
+To provide a uniform interface to functions defined via structural and well-founded recursion and to check its own correctness, the elaborator proves equational lemmas that relate the function to its original definition.
+In the function's namespace, `eq_unfold` relates the function directly to its definition, `eq_def` relates it to the definition after instantiating implicit parameters, and $`N` lemmas `eq_N` relate each case of its pattern-matching to the corresponding right-hand side, including sufficient assumptions to indicate that earlier branches were not taken.
+
+::::keepEnv
+:::example "Equational Lemmas"
+Given the definition of {lean}`thirdOfFive`:
+```lean
+def thirdOfFive : List α → Option α
+  | [_, _, x, _, _] => some x
+  | _ => none
+```
+equational lemmas are generated that relate {lean}`thirdOfFive` to its definition.
+
+{lean}`thirdOfFive.eq_unfold` states that it can be unfolded to its original definition when no arguments are provided:
+```signature
+thirdOfFive.eq_unfold.{u_1} :
+  @thirdOfFive.{u_1} = fun {α : Type u_1} x =>
+    match x with
+    | [head, head_1, x, head_2, head_3] => some x
+    | x => none
+```
+
+{lean}`thirdOfFive.eq_def` states that it matches its definition when applied to arguments:
+```signature
+thirdOfFive.eq_def.{u_1} {α : Type u_1} :
+  ∀ (x : List α),
+    thirdOfFive x =
+      match x with
+      | [head, head_1, x, head_2, head_3] => some x
+      | x => none
+```
+
+{lean}`thirdOfFive.eq_1` shows that its first defining equation holds:
+```signature
+thirdOfFive.eq_1.{u} {α : Type u}
+    (head head_1 x head_2 head_3 : α) :
+  thirdOfFive [head, head_1, x, head_2, head_3] = some x
+```
+
+{lean}`thirdOfFive.eq_2` shows that its second defining equation holds:
+```signature
+thirdOfFive.eq_2.{u_1} {α : Type u_1} :
+  ∀ (x : List α),
+    (∀ (head head_1 x_1 head_2 head_3 : α),
+      x = [head, head_1, x_1, head_2, head_3] → False) →
+    thirdOfFive x = none
+```
+The final lemma {lean}`thirdOfFive.eq_2` includes a premise that the first branch could not have matched (that is, that the list does not have exactly five elements).
+:::
+::::
+
+::::keepEnv
+:::example "Recursive Equational Lemmas"
+Given the definition of {lean}`everyOther`:
+```lean
+def everyOther : List α → List α
+  | [] => []
+  | [x] => [x]
+  | x :: _ :: xs => x :: everyOther xs
+```
+
+equational lemmas are generated that relate {lean}`everyOther`'s recursor-based implementation to its original recursive definition.
+
+{lean}`everyOther.eq_unfold` states that a fully unapplied `everyOther` is equal to its unfolding:
+```signature
+everyOther.eq_unfold.{u} :
+  @everyOther.{u} = fun {α} x =>
+    match x with
+    | [] => []
+    | [x] => [x]
+    | x :: head :: xs => x :: everyOther xs
+```
+
+{lean}`everyOther.eq_def` states that a `everyOther` is equal to its definition when applied to arguments:
+```signature
+everyOther.eq_def.{u} {α : Type u} :
+  ∀ (x : List α),
+    everyOther x =
+      match x with
+      | [] => []
+      | [x] => [x]
+      | x :: head :: xs => x :: everyOther xs
+```
+
+{lean}`everyOther.eq_1` demonstrates its first pattern:
+```signature
+everyOther.eq_1.{u} {α : Type u} : everyOther [] = ([] : List α)
+```
+
+{lean}`everyOther.eq_2` demonstrates its second pattern:
+```signature
+everyOther.eq_2.{u} {α : Type u} (x : α) : everyOther [x] = [x]
+```
+
+{lean}`everyOther.eq_3` demonstrates its final pattern:
+```signature
+everyOther.eq_3.{u} {α : Type u} (x_1 head : α) (xs : List α) :
+  everyOther (x_1 :: head :: xs) = x_1 :: everyOther xs
+```
+
+Because the patterns do not overlap, no assumptions about prior patterns not having matched are necessary for the equational lemmas.
+:::
+::::
+
+After elaborating a module, having checked each addition to the environment with the kernel, the changes that the module made to the global environment (including extensions) are serialized to a `.olean` file.
+In these files, Lean terms and values are represented just as they are in memory; thus the file can be directly memory-mapped.
+All code paths that lead to Lean adding to the environment involve the new type or definition first being checked by the kernel.
+However, Lean is a very open, flexible system.
+To guard against the possibility of poorly-written metaprograms jumping through hoops to add unchecked values to the environment, a separate tool `lean4checker` can be used to validate that the entire environment in a `.olean` file satisfies the kernel.
+
+In addition to the `.olean` file, the elaborator produces a `.ilean` file, which is an index used by the language server.
+This file contains information needed to work interactively with the module without fully loading it, such as the source positions of definitions.
+The contents of `.ilean` files are an implementation detail and may change at any release.
+
+Finally, the compiler is invoked to translate the intermediate representation of functions stored in its environment extension into C code.
+A C file is produced for each Lean module; these are then compiled to native code using a bundled C compiler.
+If the `precompileModules` option is set in the build configuration, then this native code can be dynamically loaded and invoked by Lean; otherwise, an interpreter is used.
+For most workloads, the overhead of compilation is larger than the time saved by avoiding the interpreter, but some workloads can be sped up dramatically by precompiling tactics, language extensions, or other extensions to Lean.
 
 
 # Initialization
 
-:::planned
-Describe {deftech}[initialization]
-:::
+Before starting up, the elaborator must be correctly initialized.
+Lean itself contains {deftech}[initialization] code that must be run in order to correctly construct the compiler's initial state; this code is run before loading any modules and before the elaborator is invoked.
+Furthermore, each dependency may itself contribute initialization code, _e.g._ to set up environment extensions.
+Internally, each environment extension is assigned a unique index into an array, and this array's size is equal to the number of registered environment extensions, so the number of extensions must be known in order to correctly allocate an environment.
+
+After running Lean's own builtin initializers, the module's header is parsed and the dependencies' `.olean` files are loaded into memory.
+A “pre-environment” is constructed that contains the union of the dependencies' environments.
+Next, all initialization code specified by the dependencies is executed in the interpreter.
+At this point, the number of environment extensions is known, so the pre-environment can be reallocated into an environment structure with a correctly-sized extensions array.
+
 
 :::syntax command
+An {keywordOf Lean.Parser.Command.initialize}`initialize` block adds code to the module's initializers.
+The contents of an {keywordOf Lean.Parser.Command.initialize}`initialize` block are treated as the contents of a {keywordOf Lean.Parser.Term.do}`do` block in the {lean}`IO` monad.
+
+Sometimes, initialization only needs to extend internal data structures by side effect.
+In that case the contents are expected to have type {lean}`IO Unit`:
 ```grammar
 initialize
   $cmd*
 ```
 
+Initialization may also be used to construct values that contain references to internal state, such as attributes that are backed by an environment extension.
+In this form of {keywordOf Lean.Parser.Command.initialize}`initialize`, initialization should return the specified type in the {lean}`IO` monad.
+```grammar
+initialize $x:ident : $t:term ←
+  $cmd*
+```
+:::
+
+
+:::syntax command
+Lean's internals also define code that must run during initialization.
+However, because Lean is a bootstrapping compiler, special care must be taken with initializers defined as part of Lean itself, and Lean's own initializers must run prior to importing or loading _any_ modules.
+These initializers are specified using {keywordOf Lean.Parser.Command.initialize}`builtin_initialize`, which should not be used outside the compiler's implementation.
+
+```grammar
+builtin_initialize
+  $cmd*
+```
+```grammar
+builtin_initialize $x:ident : $t:term ←
+  $cmd*
+```
 :::
