Manual/Meta.lean
@@ -12,6 +12,7 @@ import SubVerso.Examples
 
 import Manual.Meta.Attribute
 import Manual.Meta.Basic
+import Manual.Meta.Bibliography
 import Manual.Meta.CustomStyle
 import Manual.Meta.Example
 import Manual.Meta.Figure
