Manual/Meta/Bibliography.lean
@@ -1,0 +1,245 @@
+import Lean.Data.Json
+import Lean.Elab.InfoTree.Types
+
+import Verso.Output.Html
+import Verso.Output.TeX
+import VersoManual
+
+import Manual.Meta.Marginalia
+
+namespace Manual
+
+open Lean Elab
+open Verso Doc Elab Html
+open Verso.Output Html
+open Verso.Genre Manual
+open Verso.ArgParse
+
+inductive Style where
+  | textual
+  | parenthetical
+deriving ToJson, FromJson, Repr
+
+inductive Month where
+  | january | february | march | april
+  | may | june | july | august
+  | september | october | november | december
+deriving ToJson, FromJson, DecidableEq, Ord, Repr
+
+structure InProceedings where
+  title : Doc.Inline Manual
+  authors : Array (Doc.Inline Manual)
+  year : Int
+  booktitle : Doc.Inline Manual
+  editors : Option (Array (Doc.Inline Manual)) := none
+  series : Option (Doc.Inline Manual) := none
+  url : Option String := none
+deriving ToJson, FromJson, BEq, Hashable
+
+structure Thesis where
+  title : Doc.Inline Manual
+  author : Doc.Inline Manual
+  year : Int
+  university : Doc.Inline Manual
+  degree : Doc.Inline Manual
+  url : Option String := none
+deriving ToJson, FromJson, BEq, Hashable, Ord
+
+
+section
+attribute [local instance] Ord.arrayOrd
+deriving instance Ord for InProceedings
+end
+
+inductive Citable where
+  | inProceedings : InProceedings → Citable
+  | thesis : Thesis → Citable
+deriving ToJson, FromJson, BEq, Hashable, Ord
+
+instance : Coe InProceedings Citable where
+  coe := .inProceedings
+
+instance : Coe Thesis Citable where
+  coe := .thesis
+
+def Citable.authors : Citable → Array (Doc.Inline Manual)
+  | .inProceedings p => p.authors
+  | .thesis p => #[p.author]
+
+def Citable.title : Citable → Doc.Inline Manual
+  | .inProceedings p => p.title
+  | .thesis p => p.title
+
+def Citable.year : Citable → Int
+  | .inProceedings p => p.year
+  | .thesis p => p.year
+
+def Citable.url : Citable → Option String
+  | .inProceedings p => p.url
+  | .thesis p => p.url
+
+
+private def slugString : Doc.Inline Manual → String
+  | .text s | .code s | .math _ s => s
+  | .bold i | .emph i | .concat i | .other _ i | .link i _ =>
+    i.attach.map (fun ⟨x, _⟩ => slugString x) |>.foldr (init := "") (· ++ ·)
+  | .linebreak .. | .image .. | .footnote .. => ""
+
+
+def Citable.tag (c : Citable) : Slug :=
+  c.authors.map (slugString) |>.foldr (init := s!"-{c.year}") (· ++ ·) |> .ofString
+
+def Citable.sortKey (c : Citable) := c.authors.map slugString |>.foldr (init := s!" {c.year}") (· ++ ", " ++ ·)
+
+private def andList (xs : Array Html) : Html :=
+  if h : xs.size = 1 then xs[0]
+  else
+    open Html in
+    (xs.extract 0 (xs.size - 2)).foldr (init := {{" and " {{xs.back}} }}) (· ++ ", " ++ ·)
+
+partial def Bibliography.lastName (inl : Doc.Inline Manual) : Doc.Inline Manual :=
+  let ws := words inl
+  if _ : ws.size = 0 then inl
+  else if _ : ws.size = 1 then ws[0]
+  else Id.run do
+    let mut lst := #[ws.back]
+    let mut rest := ws.pop
+    while rest.back?.isSome do
+      let w := rest.back
+      rest := rest.pop
+      if parts.contains w then
+        lst := lst.push w
+        continue
+      else
+        break
+    return .concat lst.reverse
+
+where
+  parts : List (Doc.Inline Manual) := ["de", "van", "la"].map .text
+
+  words : Doc.Inline Manual → Array (Doc.Inline Manual)
+  | .text str => str.splitOn " " |>.filter (· ≠ "") |>.toArray |>.map (.text)
+  | .concat xs => xs.map words |>.foldl (init := #[]) (· ++ ·)
+  | .linebreak .. => #[]
+  | other => #[other]
+
+
+def Citable.inlineHtml
+    (go : Doc.Inline Genre.Manual → HtmlT Manual (ReaderT ExtensionImpls IO) Html)
+    (p : Citable)
+    (fmt : Style) :
+    HtmlT Manual (ReaderT ExtensionImpls IO) Html :=
+  open Html in do
+    let authors ←
+      if p.authors.size = 0 then
+        pure {{""}}
+      else if h : p.authors.size = 1 then
+        go <| Bibliography.lastName p.authors[0]
+      else if h : p.authors.size > 3 then
+        (· ++ {{<em>"et al"</em>}}) <$> go (Bibliography.lastName p.authors[0])
+      else andList <$> p.authors.mapM go
+    -- TODO disambiguate when there are duplicate author/years
+    -- TODO link to bibliography once it exists
+    match fmt with
+    | .textual =>
+      return {{ {{authors}} s!" ({p.year})"}}
+    | .parenthetical =>
+      return {{" ("{{authors}} s!", {p.year})"}}
+
+def Citable.bibHtml (go : Doc.Inline Genre.Manual → HtmlT Manual (ReaderT ExtensionImpls IO) Html) (c : Citable) : HtmlT Manual (ReaderT ExtensionImpls IO) Html := open Html in do
+  match c with
+  |  .inProceedings p =>
+    let authors ← andList <$> p.authors.mapM go
+    return {{ {{authors}} s!", {p.year}. " {{ link {{"“" {{← go p.title}} "”"}} }} ". In " <em>{{← go p.booktitle}}"."</em>{{(← p.series.mapM go).map ({{"(" {{·}} ")" }}) |>.getD .empty}} }}
+  | .thesis p =>
+    return {{ {{← go p.author}} s!", {p.year}. " <em>{{link (← go p.title)}}</em> ". " {{← go p.degree}} ", " {{← go p.university}} }}
+where
+  link (title : Html) : Html :=
+    match c.url with
+    | none => title
+    | some u => {{<a href={{u}}>{{title}}</a>}}
+
+def Inline.cite (citation : Citable) (style : Style := .parenthetical) : Inline where
+  name := `Manual.citation
+   -- The nested bit here _should_ be a no-op, but it's to avoid deserialization overhead during the traverse pass
+  data := ToJson.toJson (ToJson.toJson citation, style)
+
+structure CiteConfig where
+  citation : Name
+
+def CiteConfig.parse [Monad m] [MonadInfoTree m] [MonadLiftT CoreM m] [MonadEnv m] [MonadError m] [MonadFileMap m] : ArgParse m CiteConfig :=
+  CiteConfig.mk <$> .positional `citation .resolvedName
+
+
+@[role_expander citep]
+def citep : RoleExpander
+  | args, extra => do
+    let config ← CiteConfig.parse.run args
+    let x := mkIdent config.citation
+    return #[← `(Doc.Inline.other (Inline.cite ($x : Citable) .parenthetical) #[$(← extra.mapM elabInline),*])]
+
+@[role_expander citet]
+def citet : RoleExpander
+  | args, extra => do
+    let config ← CiteConfig.parse.run args
+    let x := mkIdent config.citation
+    return #[← `(Doc.Inline.other (Inline.cite ($x : Citable) .textual) #[$(← extra.mapM elabInline),*])]
+
+def citation := ()
+
+@[inline_extension citation]
+partial def cite.inlineDescr : InlineDescr where
+  traverse _ data _ := do
+    match FromJson.fromJson? data with
+    | .error e => logError "Failed to deserialize citation"; return none
+    | .ok (v : Json × Style) =>
+      let cited : Option (Except String (Array Json)) := (← get).get? `Manual.Bibliography
+      match cited with
+      | .none =>
+        modify (·.set `Manual.Bibliography (Json.arr #[v.1]))
+      | .some (.error e) => logError e
+      | .some (.ok citedSet) =>
+        if citedSet.binSearchContains v.1 (cmp · · == .lt) then pure ()
+        else modify (·.set `Manual.Bibliography <| citedSet.binInsert (cmp · · == .lt) v.1)
+      pure none -- TODO disambiguate years
+  toTeX := none
+  extraCss := [Marginalia.css]
+  toHtml :=
+    open Verso.Output.Html in
+    some <| fun go _ data _content => do -- TODO repurpose "content" for e.g. "page 5"
+      match FromJson.fromJson? data with
+      | .error e => HtmlT.logError s!"Failed to deserialize citation/style: {e}"; return {{""}}
+      | .ok (v : Json × Style) =>
+        match FromJson.fromJson? v.1 with
+        | .error e => HtmlT.logError s!"Failed to deserialize citation: {e}"; return {{""}}
+        | .ok (v' : Citable) =>
+          let inl ← v'.inlineHtml go v.2
+          let m ← v'.bibHtml go
+          pure <| inl ++ Marginalia.html m
+where
+  cmp : Json → Json → Ordering
+    | .null, .null => .eq
+    | .null, _ => .lt
+    | _, .null => .gt
+    | .str s1, .str s2 => Ord.compare s1 s2
+    | .str _, _ => .lt
+    | _, .str _ => .gt
+    | .num n1, .num n2 => Ord.compare n1 n2
+    | .num _, _ => .lt
+    | _, .num _ => .gt
+    | .bool b1, .bool b2 => Ord.compare b1 b2
+    | .bool _, _ => .lt
+    | _, .bool _ => .gt
+    | .arr a1, .arr a2 => (@Ord.arrayOrd _ ⟨cmp⟩).compare a1 a2
+    | .arr _, _ => .lt
+    | _, .arr _ => .gt
+    | .obj o1, .obj o2 =>
+      let inst1 : Ord String := inferInstance
+      let inst2 : Ord Json := ⟨cmp⟩
+      let inst : Ord (String × Json) := Ord.lex inst1 inst2
+      let a1 := o1.toArray.map (fun x => (x.1, x.2)) |>.qsort (inst.compare · · == .lt)
+      let a2 := o2.toArray.map (fun x => (x.1, x.2)) |>.qsort (inst.compare · · == .lt)
+      (Ord.arrayOrd).compare a1 a2
+
+
+-- TODO: Block-level element for the actual bibliography
